\begin{frame}[fragile]
\frametitle{Combining Functors}
\begin{block}{Mapping on a [] of Maybe}
Suppose I glue two functors, \lstinline$[]$ and \lstinline$Maybe$, together:
\begin{lstlisting}[language=haskell]
  value :: [Maybe a]
\end{lstlisting}
and I want to map a function \lstinline$f :: a -> b$:
\begin{lstlisting}[language=haskell]
  result :: [Maybe b]
  result = fmap (fmap f) value
\end{lstlisting}
\end{block}
\end{frame}

\begin{frame}[fragile]
\frametitle{Functor Composition}
\begin{block}{Mapping on a (f of g)}
\begin{lstlisting}[language=haskell]
  \f -> fmap (fmap f) ::
    (Functor f, Functor g) =>
    (a -> b) -> f (g a) -> f (g b)
\end{lstlisting}
\end{block}
\end{frame}

\begin{frame}[fragile]
\frametitle{Functor Composition}
\begin{block}{Mapping on a (f of g)}
In fact, I can do this for any two functors:
\begin{lstlisting}[language=haskell]
  value :: f (g a)
\end{lstlisting}
to map a function \lstinline$f :: a -> b$:
\begin{lstlisting}[language=haskell]
  result :: f (g b)
  result = fmap (fmap f) value
\end{lstlisting}
\end{block}
\end{frame}

\begin{frame}[fragile]
\frametitle{Functor Composition}
\begin{block}{In other words}
If f and g are functors, then (f of g) is a functor:
\begin{lstlisting}[language=haskell]
  data Compose f g x = Compose (f (g x))

  instance (Functor f, Functor g) =>
      Functor (Compose f g) where
    fmap f (Compose z) =
      Compose (fmap (fmap f) z)
\end{lstlisting}
\end{block}
\end{frame}

\begin{frame}
\frametitle{Functors Compose}
The composition of two arbitrary functors makes a new functor.

In brief, we say that \emph{functors compose}.
\end{frame}
